Add back wf assumptions -Also prove two lemmas that might be useful to remove it again

compiler/backend/proofs/word_to_stackProofScript.sml
@@ -552,6 +552,7 @@ val state_rel_def = Define `
     1 ≤ LENGTH t.bitmaps ∧ HD t.bitmaps = 4w ∧
     t.stack_space + f <= LENGTH t.stack /\ LENGTH t.stack < dimword (:'a) /\
     (if f' = 0 then f = 0 else (f = f' + 1)) /\
+    wf s.locals /\
     let stack = DROP t.stack_space t.stack in
     (*First f things on stack are the live stack vars*)
     let current_frame = TAKE f stack in
@@ -969,6 +970,7 @@ val evaluate_wLive = Q.prove(
     \\ match_mp_tac (GSYM DROP_list_LUPDATE_IGNORE |> Q.SPEC `[x]`
            |> SIMP_RULE std_ss [list_LUPDATE_def])
     \\ fs [] \\ decide_tac)
+  \\ fs[wf_def]
   \\ fs [stack_rel_def,stack_rel_aux_def,abs_stack_def]
   \\ Cases_on `DROP t.stack_space t.stack` \\ fs []
   THEN1 (fs [listTheory.DROP_NIL,DECIDE ``m>=n<=>n<=m:num``] \\ `F` by decide_tac)
@@ -1625,6 +1627,7 @@ val alloc_IMP_alloc = prove(
       (imp_res_tac dec_stack_length>>
       fs[LENGTH_DROP]>>
       DECIDE_TAC)>>
+    simp[wf_fromAList] >>
     CONJ_TAC>-
       (fs[stack_rel_def,LET_THM]>>
       qpat_assum`abs_stack A B C D = E` mp_tac>>
@@ -2240,7 +2243,7 @@ val state_rel_set_var = Q.store_thm("state_rel_set_var",
     state_rel k f f' (set_var (2*x) v s) (set_var x v t) lens`,
   simp[state_rel_def,stackSemTheory.set_var_def,wordSemTheory.set_var_def]
   \\ strip_tac
-  \\ fs[lookup_insert,FLOOKUP_UPDATE]
+  \\ fs[lookup_insert,FLOOKUP_UPDATE,wf_insert]
   \\ rpt gen_tac
   \\ IF_CASES_TAC \\ simp[]
   >- (
@@ -2260,7 +2263,7 @@ val state_rel_set_var2 = Q.store_thm("state_rel_set_var2",
     (t with stack := LUPDATE v (sp + (f + k − (x + 1))) st) lens`,
   simp[state_rel_def,stackSemTheory.set_var_def,wordSemTheory.set_var_def]
   \\ strip_tac
-  \\ fs[lookup_insert,FLOOKUP_UPDATE]
+  \\ fs[lookup_insert,FLOOKUP_UPDATE,wf_insert]
   \\ simp[DROP_LUPDATE]
   \\ rpt gen_tac
   \\ IF_CASES_TAC \\ simp[]
@@ -3398,6 +3401,41 @@ val ALOOKUP_ID_TABULATE = Q.store_thm("ALOOKUP_ID_TABULATE",
    if MEM x ls then SOME x else NONE`,
   Induct_on`ls`\\simp[]\\rw[]\\fs[]);
 
+(*These two might be used to remove wf assumption if needed*)
+val insert_unchanged = prove(``
+  ∀t x.
+  lookup x t = SOME y ⇒
+  insert x y t = t``,
+  completeInduct_on`x`>>
+  Induct>>
+  fs[lookup_def]>>rw[]>>
+  simp[Once insert_def,SimpRHS]>>
+  simp[Once insert_def]>>
+  imp_res_tac splem1>>
+  metis_tac[])
+
+val alist_insert_ALL_DISTINCT = prove(``
+  ∀xs ys t ls.
+  ALL_DISTINCT xs ∧
+  LENGTH xs = LENGTH ys ∧
+  PERM (ZIP (xs,ys)) ls ⇒
+  alist_insert xs ys t = alist_insert (MAP FST ls) (MAP SND ls) t``,
+  ho_match_mp_tac alist_insert_ind>>rw[]>>
+  fs[LENGTH_NIL_SYM]>>rveq>>fs[ZIP]>>
+  simp[alist_insert_def]>>
+  fs[PERM_CONS_EQ_APPEND]>>
+  simp[alist_insert_append,alist_insert_def]>>
+  `¬MEM xs (MAP FST M)` by
+    (CCONTR_TAC>>fs[]>>
+    imp_res_tac PERM_MEM_EQ>>
+    fs[FORALL_PROD,MEM_MAP,EXISTS_PROD]>>
+    res_tac>>
+    imp_res_tac MEM_ZIP>>
+    fs[EL_MEM])>>
+  simp[alist_insert_pull_insert]>>
+  simp[GSYM alist_insert_append]>>
+  metis_tac[MAP_APPEND])
+
 val alist_insert_get_vars = Q.store_thm("alist_insert_get_vars",
   `∀moves s x ls.
    ALL_DISTINCT (MAP FST moves) ∧
@@ -3710,7 +3748,7 @@ val comp_correct = Q.store_thm("comp_correct",
     \\ conj_tac >- fs[parmoveTheory.windmill_def]
     \\ simp[]
     \\ conj_tac >- metis_tac[ALL_DISTINCT_parmove]
-    \\ conj_tac >- cheat (* need wf s.locals in state *)
+    \\ conj_tac >- fs[state_rel_def]
     \\ conj_tac >- metis_tac[MEM_MAP_FST_parmove]
     \\ metis_tac[parmove_preserves_moves])
   THEN1 (* Inst *) cheat
@@ -3791,7 +3829,7 @@ val comp_correct = Q.store_thm("comp_correct",
       \\ fs [state_rel_def,empty_env_def,call_env_def,LET_DEF,
              fromList2_def,lookup_def]
       \\ fs [AC ADD_ASSOC ADD_COMM]
-      \\ imp_res_tac DROP_DROP \\ fs [])
+      \\ imp_res_tac DROP_DROP \\ fs [wf_def])
     \\ `~(LENGTH t.stack < t.stack_space + (f -1 - (n DIV 2 - k))) /\
         (EL (t.stack_space + (f -1 - (n DIV 2 - k))) t.stack = Loc l1 l2) /\
         (get_var 1 t = SOME x')` by
@@ -3814,7 +3852,7 @@ val comp_correct = Q.store_thm("comp_correct",
     \\ fs [state_rel_def,empty_env_def,call_env_def,LET_DEF,
            fromList2_def,lookup_def]
     \\ fs [AC ADD_ASSOC ADD_COMM]
-    \\ imp_res_tac DROP_DROP \\ fs [])
+    \\ imp_res_tac DROP_DROP \\ fs [wf_def])
   THEN1 (* Raise *)
    (fs [wordSemTheory.evaluate_def,jump_exc_def]
     \\ `1 < k` by (fs [state_rel_def] \\ decide_tac)
@@ -3869,7 +3907,7 @@ val comp_correct = Q.store_thm("comp_correct",
     discharge_hyps >- simp[]>>
     rw[] >>
     fs [FLOOKUP_UPDATE]>>
-    rfs[]
+    rfs[wf_def]
     \\ conj_tac THEN1
      (fs [sorted_env_def] \\ Cases_on `env_to_list (fromAList l) (K I)`
       \\ imp_res_tac env_to_list_K_I_IMP \\ fs [])
@@ -3910,6 +3948,8 @@ val comp_correct = Q.store_thm("comp_correct",
           fs [state_rel_def] \\ fs [LET_THM]
     \\ qexists_tac `0` \\ fs []
     \\ fs [state_rel_def,LET_THM]
+    \\ conj_tac
+    >- ( fs[cut_env_def] \\ rveq \\ simp[wf_inter] )
     \\ ntac 3 strip_tac
     \\ fs [cut_env_def] \\ rpt var_eq_tac
     \\ fs [lookup_inter_alt]
@@ -4343,7 +4383,7 @@ val init_state_ok_IMP_state_rel = prove(
   \\ fs [stack_rel_def,sorted_env_def,abs_stack_def,LET_THM]
   \\ fs [handler_val_def,LASTN_def,stack_rel_aux_def]
   \\ fs [filter_bitmap_def,MAP_FST_def,index_list_def]
-  \\ fs[flookup_thm] \\ every_case_tac \\ fs [] \\ decide_tac);
+  \\ fs[flookup_thm,wf_def] \\ every_case_tac \\ fs [] \\ decide_tac);
 
 val init_state_ok_semantics =
   state_rel_IMP_semantics |> Q.INST [`s`|->`make_init t code`]
